moving stuff around, reducibility, cleaning a bit

theories/lam/wkpre.v
@@ -1,8 +1,8 @@
 From iris.program_logic Require Import language ectxi_language ectx_language lifting.
 From iris Require Import program_logic.weakestpre.
 From iris.proofmode Require Import tactics.
-From st.lam Require Import lang tactics.
 From st.prelude Require Import at_least_one.
+From st.lam Require Import lang reducibility.
 
 Section wkpre_lemmas.
 
@@ -45,72 +45,17 @@ Section wkpre_lemmas.
     by iApply wp_rtc_steps.
   Qed.
 
-  (* things with stuckness *)
-  Definition lam_head_step (e e' : expr) := head_step e tt [] e' tt [].
-
-  Lemma head_to_lam_head (e e' : expr) σ σ' κ efs : head_step e σ κ e' σ' efs → lam_head_step e e'.
-  Proof. intro H. rewrite /lam_head_step. inversion H; by econstructor. Qed.
-
-  Definition lam_reducible (e : expr) := ∃ e', lam_step e e'.
-
-  Definition lam_irreducible (e : expr) := ∀ e', ¬ lam_step e e'.
-
-  Lemma prim_to_lam (e1 e2 : expr) σ1 σ2 κ efs : prim_step e1 σ1 κ e2 σ2 efs -> lam_step e1 e2.
-  Proof. intro H. apply lam_pure. apply (prim_step_pure _ _ _ _ _ _ H). Qed.
-
-  Lemma lam_prim_red (e : expr) : lam_reducible e <-> reducible e tt.
-  Proof.
-    split. intro H. destruct H as [e' Hstep]. exists [], e', tt, []. apply Hstep.
-    intro H. destruct H as (a & e' & b & c & Hstep). exists e'. by eapply prim_to_lam.
-  Qed.
-
-  Definition lam_head_reducible (e : expr) := ∃ e', lam_head_step e e'.
-  Definition lam_head_irreducible (e : expr) := ∀ e', ¬ lam_head_step e e'.
-
-  Lemma lam_head_red_iff_head_red (e : expr) : lam_head_reducible e <-> head_reducible e tt.
-  Proof.
-    split. intro H. destruct H as [e' Hstep]. exists [], e', tt, []. apply Hstep.
-    intro H. destruct H as (a & e' & b & c & Hstep). exists e'. destruct Hstep; by econstructor.
-  Qed.
-
-  Lemma lam_head_irred_iff_head_irred (e : expr) : lam_head_irreducible e <-> head_irreducible e tt.
-  Proof.
-    split. intro H. intros κ e' σ efs abs. apply (H e'). by eapply head_to_lam_head.
-    intros H e' Hstep. apply (H [] e' () []). auto.
-  Qed.
-
-  Instance dec_expr_reducible (e : expr) : Decision (reducible e tt).
-  Proof.
-  Admitted.
-
   Lemma wp_Maybestuck_True (e : expr) : ⊢ WP e ? {{ v , True }}.
   Proof.
     revert e. iLöb as "H". iIntros (e).
-    destruct (decide (reducible e tt)).
-    - destruct r as [aa [e' [cc [dd Hstep]]]].
-      destruct cc.
-      assert (dd = []) as eq. by eapply prim_step_no_forks. rewrite eq in Hstep.
-      assert (aa = []) as eq1. by eapply prim_step_no_obs. rewrite eq1 in Hstep.
-      iApply wp_step_later. apply Hstep. iNext. iApply "H".
-    - destruct (decide (to_val e = None)).
-      iApply wp_lift_pure_stuck. intro σ. destruct σ. split; auto. by apply not_reducible. auto.
-      destruct (to_val e) eqn:eq. iApply (wp_value _ _ _ _ v). eapply of_to_val; fast_done. auto.
-      contradiction.
+    destruct (dec_expr_reducibility e) as [v1 eq1 | is_red1 | is_stuck1 ]; first rewrite -(of_to_val _ _ eq1).
+    - by iApply wp_value'.
+    - assert (is_red : lam_reducible e) by by apply lam_prim_red. destruct is_red as [e' Hs].
+      iApply wp_step_later. apply Hs. iNext. iApply "H".
+    - iApply wp_lift_pure_stuck; auto. by intro σ; destruct σ.
   Qed.
 
   Lemma wp_stuck Φ (e : expr) (H : stuck e tt) : ⊢ WP e ?{{ v, Φ v }}.
   Proof. apply wp_lift_pure_stuck. intro σ. by destruct σ. Qed.
 
 End wkpre_lemmas.
-
-Ltac head_stuck_solver :=
-  lazymatch goal with
-  | |- stuck ?e () => apply head_stuck_stuck; head_stuck_solver
-  | |- head_stuck ?e () => split; head_stuck_solver
-  | |- rtc lam_step _ _ => (eapply rtc_l; first (auto_lam_step); simplify_custom)
-  | |- ectx_language.to_val _ = _ => (by simplify_custom) ; head_stuck_solver
-  | |- head_irreducible _ () => ((apply lam_head_irred_iff_head_irred; intros e' abs; inversion abs; simplify_option_eq); try done); head_stuck_solver
-  | |- sub_redexes_are_values _ => apply ectxi_language_sub_redexes_are_values; intros Ki' e' eq; destruct Ki'; inversion eq; head_stuck_solver
-  | |- is_Some _ => (by eexists; simplify_custom) ; head_stuck_solver
-  | |- _ => auto
-  end.
