theories/backtranslations/sem_syn/connective/nr_syn_le_un.v
@@ -3,8 +3,9 @@ From iris.proofmode Require Import tactics.
 From iris_string_ident Require Import ltac2_string_ident.
 From st.prelude Require Import autosubst.
 From st.lam Require Import wkpre types nr_types lang typing tactics logrel.definitions logrel.generic.lift.
-From st.lam.lib Require Import fixlam universe.nr_embed_project universe.base.
+From st.backtranslations.un_syn Require Import universe.base.
 From st.backtranslations.un_syn.logrel Require Import definitions syn_le_un.fundamental.
+From st.backtranslations.sem_syn Require Import nr_embed_project.
 
 (* Defines connective lemma between the untyped and typed logic relations (the (syntactically typed ≤ untyped)-refinement) *)
 (* Of the two refinements, this is the easier one *)
