theories/backtranslations/sem_syn/connective/nr_un_le_syn.v
@@ -2,9 +2,9 @@ From iris Require Import program_logic.weakestpre.
 From iris.proofmode Require Import tactics.
 From iris_string_ident Require Import ltac2_string_ident.
 From st.prelude Require Import autosubst big_op_three.
-From st.lam.lib Require Import fixlam universe.nr_embed_project nr_guard_assert universe.base universe.paths.
 From st.lam Require Import wkpre types nr_types lang typing tactics logrel.definitions logrel.generic.lift.
-From st.backtranslations.un_syn Require Import logrel.definitions logrel.un_le_syn.fundamental.
+From st.backtranslations.un_syn Require Import logrel.definitions logrel.un_le_syn.fundamental universe.base universe.paths.
+From st.backtranslations.sem_syn Require Import nr_embed_project nr_guard_assert.
 
 (* Defines connective lemma between the untyped and typed logic relations (the (untyped ≤ syntactically typed)-refinement) *)
 (* Of the two refinements, this is the harder one; we need the additional guards/asserts *)
