theories/backtranslations/sem_syn/nr_embed_project.v
@@ -1,6 +1,6 @@
 From st.prelude Require Import autosubst.
 From st.lam Require Import types nr_types lang typing tactics.
-From st.lam.lib Require Import fixlam omega universe.base.
+From st.backtranslations.un_syn Require Import universe.base.
 
 Inductive direction :=
   | Embed
