theories/backtranslations/st_sem/well_defined/logrel/fundamental.v
@@ -1,10 +1,9 @@
 From iris Require Import program_logic.weakestpre.
 From st.lamst Require Import lang types typing.
 From st.lam Require Import lang wkpre generic.lift.
-From st.backtranslations.st_sem Require Import ghost heap expressions.
-From st.backtranslations.st_sem.well_defined.logrel Require Import definition.
+From st.backtranslations.st_sem Require Import ghost heap_emul.base expressions.
+From st.backtranslations.st_sem.well_defined.logrel Require Import definition compat_lemmas.
 From iris.proofmode Require Import tactics.
-Require Import compat_lemmas.
 
 Section fundamental_theorem.
 
@@ -37,34 +36,13 @@ Section fundamental_theorem.
     - admit.
     - admit.
     - admit.
-      (* !! intersting ones !! *)
+    - by apply compat_alloc.
+    - by apply compat_read.
+    - by eapply compat_write.
+    - by eapply compat_bind.
+    - by apply compat_retrn.
+    - by apply compat_runst.
+    - by eapply compat_equal.
+  Admitted.
 
-    - (* alloc *)
-      (* cleaning and getting to the gist of it *)
-      iIntros (Δ vs vs') "#Hvsvs'".
-      specialize (IHd Δ vs vs').
-      iDestruct (IHd with "Hvsvs'") as "Hee'". clear IHd. iClear "Hvsvs'".
-      admit.
-    - (* read *)
-      (* cleaning and getting to the gist of it *)
-      iIntros (Δ vs vs') "#Hvsvs'".
-      specialize (IHd Δ vs vs').
-      iDestruct (IHd with "Hvsvs'") as "Hee'". clear IHd. iClear "Hvsvs'".
-      admit.
-    - (* write *)
-      (* cleaning and getting to the gist of it *)
-      iIntros (Δ vs vs') "#Hvsvs'".
-      specialize (IHd1 Δ vs vs').
-      iDestruct (IHd1 with "Hvsvs'") as "Hee'". clear IHd1.
-      specialize (IHd2 Δ vs vs'). clear IHd2.
-      iClear "Hvsvs'".
-      admit.
-    - (* bind *)
-      admit.
-    - (* return *)
-      admit.
-    - (* runst *)
-      admit.
-    - (* equal *)
-      admit.
-
+End fundamental_theorem.
