theories/lam/lib/dummy.v
@@ -1,4 +1,0 @@
-From st.lam Require Import lang.
-
-Definition dummy : expr.
-Proof. exact ()%Eₙₒ. Qed.
