theories/lam/tactics.v
@@ -199,7 +199,6 @@ Ltac auto_rtc_lam_step :=
   | |- _ => fail "Goal not a rtc lam_step"
   end.
 
-
 (* Hint Extern 5 (IntoVal _ _) => eapply of_to_val; fast_done : typeclass_instances. *)
 (* Hint Extern 10 (IntoVal _ _) => *)
 (*   rewrite /IntoVal; eapply of_to_val; rewrite /= !to_of_val /=; solve [ eauto ] : typeclass_instances. *)
